---
quickshare-date: 2024-09-01 22:36:22
quickshare-url: "https://noteshare.space/note/cm0jsn7fh2708601mwvsvtvn33#kqdJ1eBRA7kqjLr9H9wPALfZAbQZnb92lpX7bNWr444"
dg-publish: true
---

## Rotation | Transformation of axis

- The equation of $xy$ coordinate system:
	- $\color{yellow}ax^2+2hxy+by^2=0$
	- The relation between $xy$ and $x'y'$ coordinate systems:
		- $x =x'cos\theta-y'sin\theta$
		- $y = x'sin\theta+y'cos\theta$

<font color="#ffff00">From the equation putting the values</font>
$=> a(x'cos\theta-y'sin\theta)^2+2h(x'cos\theta-y'sin\theta)(x'sin\theta+y'cos\theta)+b(x'sin\theta+y'cos\theta)^2=a'x'^2+2h'x'y'+'by'^2$

$\small =>xâ€²^2(acos^2Î¸+2hsinÎ¸cosÎ¸+bsin^2Î¸)+2xâ€²yâ€²(h(cos^2Î¸âˆ’sin^2Î¸)âˆ’(a-b)cosÎ¸sinÎ¸)+yâ€²^2(asin^2Î¸âˆ’2hsinÎ¸cosÎ¸+bcos^2Î¸)=a'x'^2+2h'x'y'+b'y'^2$

Equating the coefficient of $x'^2,2x'y',y'^2$ on both sides:
$\color{orange}a'=a \cos^2\theta + 2h \sin\theta \cos\theta + b \sin^2\theta$
$\color{orange}h' = h (cos^2\theta - sin^2\theta) - (a - b) cos\theta sin\theta$
$\color{orange} b'= a \sin^2\theta - 2h \sin\theta \cos\theta + b \cos^2\theta$

### To make a Standard from equation from general equation
ðŸ”´ <span style="background:rgba(0, 164, 255, 0.72); color:black">Find the angle through which the axis are to be rotated</span>. That the expression is transformed into on expression not containing the $xy$ term.

â­• $xy$ term will be vanished if:
$$h'=0$$
$$=>h(cos\theta^2-sin\theta^2)-(a-b)sin\theta.cos\theta = 0$$
$$=>hcos2\theta-\frac{(a-b)}{2}sin2\theta=0$$
$$=>\frac{sin2\theta}{cos2\theta}=\frac{2h}{a-b}$$
$$\color{red}tan2\theta=\frac{2h}{a-b}$$
$$\color{red}=>\theta=\frac{1}{2}tan^{-1}\frac{2h}{a-b}$$

#### Invariants:
1. $a+b=a'+b'$
2. $ab-h^2=a'b'-h^2$ 